---
layout: post
title: "Q088 Merge Sorted Array"
date: 2015-05-07
tags: Two_Pointers Array
categories: Leetcode
published: true

---

## [Merge Sorted Array](https://leetcode.com/problems/merge-sorted-array/) 

### Solution 1 Recursively

#### Idea:
Recursively deal with the last element in two arrays

#### Time Complexity:
O(m+n)

#### Space Complexity:
O(1)

##### Explanation:
[Tail calls] can be implemented without adding a new stack frame to the call stack. Most of the frame of the current procedure is not needed any more, and it can be replaced by the frame of the tail call, modified as appropriate (similar to overlay for processes, but for function calls). The program can then jump to the called subroutine. 

In the following code, merge() is a tail call. It will not add additional stack, so the space complexity is O(1).

[Tail calls]: link: http://en.wikipedia.org/wiki/Tail_call

#### Source code:
{% highlight C++ %}
    void merge(int A[], int m, int B[], int n) {
        if (n == 0)
            return ;
        if (m == 0){
            for (int i = 0; i < n; i++)
                A[i] = B[i];
            return ;
        }
        if (A[m - 1] < B[n - 1]){
            A[m + n - 1] = B[n - 1];
            merge(A, m, B, n - 1);
        }
        else{
            A[m + n - 1] = A[m - 1];
            merge(A, m - 1, B, n);
        }
    }
{% endhighlight %}

---

### Solution 2

#### Idea:
Loop version of the above solution.

#### Time Complexity:
O(m + n)

#### Space Complexity:
O(1) 

#### Source code:
{% highlight C++ %}
    void merge(int A[], int m, int B[], int n) {
        int i, j;
        for (int k = m + n - 1, i = m - 1, j = n - 1; k >= 0; k--){
            if (i >= 0 && j >=0){
                if (A[i] > B[j]){
                    A[k] = A[i];
                    i--;
                }
                else{
                    A[k] = B[j];
                    j--;
                }
            }
            else if (i < 0){
                while (j >= 0){
                    A[k--] = B[j--];
                }
            }
        }
    }
{% endhighlight %}

---

**A conciser version**

{% highlight C++ %}

class Solution {
public:
    void merge(int A[], int m, int B[], int n) {
        int total=m+n;
        while(m && n)
        {
            if(A[m-1]>B[n-1]) A[--total]=A[--m];
            else A[--total]=B[--n];
        }
        while(n) A[--total]=B[--n];
    }
};

{% endhighlight %}

---

**One Line version**

{% highlight C++ %}

class Solution {
public:
    void merge(int A[], int m, int B[], int n) {
        while(n>0) A[m+n-1] = (m==0||B[n-1] > A[m-1]) ? B[--n] : A[--m];
    }
};

{% endhighlight %}
